[WIP] More Semantics

theories/Languages/Lustre.v
@@ -366,6 +366,9 @@ Inductive sem_exp (h: history) | : nat -> forall {ty}, exp ty -> value ty -> Pro
     sem_exp (S t) e2 v -> sem_exp (S t) (EBinop Bop_arrow e1 e2) v
 .
 
+Definition sem_node (n: node) (h: history) : Prop :=
+  forall (i: ident) (ty: type) (e: exp ty) (s: Stream.t (value ty)), In (i, existT _ _ e) n.(n_body) -> h_maps_to i s h -> forall n, sem_exp h n e (Stream.nth n s).
+
 
 (** ** Properties *)
 
