theories/Translations/LustreToTiming.v
@@ -2,7 +2,7 @@ Set Default Goal Selector "!".
 
 From Reactive.Languages Require Lustre LustreTiming.
 From Reactive.Languages Require Import Semantics.
-From Reactive.Props Require Import Freshness Identifier Permutations.
+From Reactive.Props Require Import Freshness Identifier Inclusion Permutations.
 
 From Stdlib Require Import List Nat Permutation.
 From Stdlib.Arith Require Import PeanoNat.
@@ -60,46 +60,52 @@ Definition translate_expr {ty} (e: Source.exp ty) (seed: ident): (
   ) :=
     Target.raw_to_comb (expr_to_raw e) seed.
 
-Lemma translate_expr_nextseed {ty} {e: Source.exp ty} {ei es: Target.comb_exp ty} {seed seed': ident} {pre_binders: list binder} {pre_eqs init_post step_post: list Target.equation}:
-  translate_expr e seed = (ei, es, seed', pre_binders, pre_eqs, init_post, step_post)
-  -> exists n, seed' = iter n next_ident seed.
+Lemma translate_expr_nextseed {ty} (e: Source.exp ty) (seed: ident):
+  let '(ei, es, seed', pre_binders, pre_eqs, init_post, step_post) :=  translate_expr e seed in
+  exists n, seed' = iter n next_ident seed.
 Proof.
-  apply Target.raw_to_comb_nextseed.
+  destruct (translate_expr e seed) as [[[[[[]]]]]] eqn: translation.
+  apply (Target.raw_to_comb_nextseed translation).
 Qed.
 
-Lemma freshness_translate_expr {ty} {e: Source.exp ty} {ei es: Target.comb_exp ty} {seed seed': ident} {pre_binders: list binder} {pre_eqs init_post step_post: list Target.equation}:
-  translate_expr e seed = (ei, es, seed', pre_binders, pre_eqs, init_post, step_post)
-  -> freshness seed' pre_binders.
+Lemma freshness_translate_expr {ty} (e: Source.exp ty) (seed: ident):
+  let '(ei, es, seed', pre_binders, pre_eqs, init_post, step_post) := translate_expr e seed in
+  freshness seed' pre_binders.
 Proof.
-  apply Target.freshness_raw_to_comb.
+  destruct (translate_expr e seed) as [[[[[[]]]]]] eqn: translation.
+  apply (Target.freshness_raw_to_comb translation).
 Qed.
 
-Lemma isnext_translate_expr {ty} {e: Source.exp ty} {ei es: Target.comb_exp ty} {seed seed': ident} {pre_binders: list binder} {pre_eqs init_post step_post: list Target.equation}:
-  translate_expr e seed = (ei, es, seed', pre_binders, pre_eqs, init_post, step_post)
-  -> forall x, In x (map fst pre_binders) -> exists n, x = iter n next_ident seed.
+Lemma isnext_translate_expr {ty} (e: Source.exp ty) (seed: ident):
+  let '(ei, es, seed', pre_binders, pre_eqs, init_post, step_post) := translate_expr e seed in
+  forall x, In x (map fst pre_binders) -> exists n, x = iter n next_ident seed.
 Proof.
-  apply Target.isnext_raw_to_comb.
+  destruct (translate_expr e seed) as [[[[[[]]]]]] eqn: translation.
+  apply (Target.isnext_raw_to_comb translation).
 Qed.
 
-Lemma nodup_translate_expr {ty} {e: Source.exp ty} {ei es: Target.comb_exp ty} {seed seed': ident} {pre_binders: list binder} {pre_eqs init_post step_post: list Target.equation}:
-  translate_expr e seed = (ei, es, seed', pre_binders, pre_eqs, init_post, step_post)
-  -> NoDup (map fst pre_binders).
+Lemma nodup_translate_expr {ty} (e: Source.exp ty) (seed: ident):
+  let '(ei, es, seed', pre_binders, pre_eqs, init_post, step_post) := translate_expr e seed in
+  NoDup (map fst pre_binders).
 Proof.
-  apply Target.nodup_raw_to_comb.
+  destruct (translate_expr e seed) as [[[[[[]]]]]] eqn: translation.
+  apply (Target.nodup_raw_to_comb translation).
 Qed.
 
-Lemma translate_expr_assigned_init {ty} {e: Source.exp ty} {ei es: Target.comb_exp ty} {seed seed': ident} {pre_binders: list binder} {pre_eqs init_post step_post: list Target.equation}:
-  translate_expr e seed = (ei, es, seed', pre_binders, pre_eqs, init_post, step_post)
-  -> Permutation (map Target.equation_dest (pre_eqs ++ init_post)) pre_binders.
+Lemma translate_expr_assigned_init {ty} (e: Source.exp ty) (seed: ident):
+  let '(ei, es, seed', pre_binders, pre_eqs, init_post, step_post) := translate_expr e seed in
+  Permutation (map Target.equation_dest (pre_eqs ++ init_post)) pre_binders.
 Proof.
-  apply Target.raw_to_comb_assigned_init.
+  destruct (translate_expr e seed) as [[[[[[]]]]]] eqn: translation.
+  apply (Target.raw_to_comb_assigned_init translation).
 Qed.
 
-Lemma translate_expr_assigned_step {ty} {e: Source.exp ty} {ei es: Target.comb_exp ty} {seed seed': ident} {pre_binders: list binder} {pre_eqs init_post step_post: list Target.equation}:
-  translate_expr e seed = (ei, es, seed', pre_binders, pre_eqs, init_post, step_post)
-  -> Permutation (map Target.equation_dest (pre_eqs ++ step_post)) pre_binders.
+Lemma translate_expr_assigned_step {ty} (e: Source.exp ty) (seed: ident):
+  let '(ei, es, seed', pre_binders, pre_eqs, init_post, step_post) := translate_expr e seed in
+  Permutation (map Target.equation_dest (pre_eqs ++ step_post)) pre_binders.
 Proof.
-  apply Target.raw_to_comb_assigned_step.
+  destruct (translate_expr e seed) as [[[[[[]]]]]] eqn: translation.
+  apply (Target.raw_to_comb_assigned_step translation).
 Qed.
 
 Fixpoint translate_equations (eqs: list Source.equation) (seed: ident): (
@@ -135,11 +141,11 @@ Fixpoint translate_equations (eqs: list Source.equation) (seed: ident): (
             )
     end.
 
-Lemma translate_equations_nextseed {eqs: list Source.equation} {seed seed': ident} {pre_binders: list binder} {init_eqs step_eqs pre_eqs init_post step_post: list Target.equation}:
-  translate_equations eqs seed = (init_eqs, step_eqs, seed', pre_binders, pre_eqs, init_post, step_post)
-  -> exists n, seed' = iter n next_ident seed.
+Lemma translate_equations_nextseed (eqs: list Source.equation) (seed: ident):
+  let '(init_eqs, step_eqs, seed', pre_binders, pre_eqs, init_post, step_post) := translate_equations eqs seed in
+  exists n, seed' = iter n next_ident seed.
 Proof.
-  intro translation.
+  destruct (translate_equations eqs seed) as [[[[[[init_eqs step_eqs] seed'] pre_binders] pre_eqs] init_post] step_post] eqn: translation.
   induction eqs as [| eq eqs IH] in seed, seed', pre_binders, init_eqs, step_eqs, pre_eqs, init_post, step_post, translation |- *.
   - injection translation as <- <- <- <- <- <- <-.
     exists 0.
@@ -147,11 +153,11 @@ Proof.
   - simpl in translation.
     destruct (translate_equations eqs seed) as [[[[[[init_eqs0 step_eqs0] seed0] binders0] pre_eqs0] init_post0] step_post0] eqn: unfoldtrans.
     destruct eq as [ident [ty expr]].
-    destruct (translate_expr expr seed0) as [[[[[[ei2 es2] seed2] binders2] pre_eqs2] init_post2] step_post2] eqn: unfoldexpr.
+    specialize (translate_expr_nextseed expr seed0) as unfoldseed.
+    destruct (translate_expr expr seed0) as [[[[[[ei2 es2] seed2] binders2] pre_eqs2] init_post2] step_post2].
     injection translation as <- <- <- <- <- <- <-.
     specialize (IH _ _ _ _ _ _ _ _ unfoldtrans).
-    apply translate_expr_nextseed in unfoldexpr.
-    destruct unfoldexpr as [nexpr seedexpr].
+    destruct unfoldseed as [nexpr seedexpr].
     destruct IH as [nIH IH].
     rewrite IH in seedexpr.
     rewrite <- Nat.iter_add in seedexpr.
@@ -159,11 +165,11 @@ Proof.
     assumption.
 Qed.
 
-Lemma freshness_translate_equations {eqs: list Source.equation} {seed seed': ident} {pre_binders: list binder} {init_eqs step_eqs pre_eqs init_post step_post: list Target.equation}:
-  translate_equations eqs seed = (init_eqs, step_eqs, seed', pre_binders, pre_eqs, init_post, step_post)
-  -> freshness seed' pre_binders.
+Lemma freshness_translate_equations (eqs: list Source.equation) (seed: ident):
+  let '(init_eqs, step_eqs, seed', pre_binders, pre_eqs, init_post, step_post) := translate_equations eqs seed in
+  freshness seed' pre_binders.
 Proof.
-  intro translation.
+  destruct (translate_equations eqs seed) as [[[[[[init_eqs step_eqs] seed'] pre_binders] pre_eqs] init_post] step_post] eqn: translation.
   induction eqs as [| eq eqs IH] in seed, seed', pre_binders, init_eqs, step_eqs, pre_eqs, init_post, step_post, translation |- *.
   - injection translation as <- <- <- <- <- <- <-.
     intro n.
@@ -171,34 +177,34 @@ Proof.
   - simpl in translation.
     destruct (translate_equations eqs seed) as [[[[[[init_eqs0 step_eqs0] seed0] binders0] pre_eqs0] init_post0] step_post0] eqn: unfoldtrans.
     destruct eq as [ident [ty expr]].
-    destruct (translate_expr expr seed0) as [[[[[[ei2 es2] seed2] binders2] pre_eqs2] init_post2] step_post2] eqn: unfoldexpr.
+    assert (freshness_expr := freshness_translate_expr expr seed0).
+    assert (nextseed_expr := translate_expr_nextseed expr seed0).
+    destruct (translate_expr expr seed0) as [[[[[[ei2 es2] seed2] binders2] pre_eqs2] init_post2] step_post2].
     injection translation as <- <- <- <- <- <- <-.
     specialize (IH _ _ _ _ _ _ _ _ unfoldtrans).
-    assert (freshness_expr := freshness_translate_expr unfoldexpr).
-    assert (nextseed_expr := translate_expr_nextseed unfoldexpr).
     apply (freshness_later_e nextseed_expr) in IH.
     apply (freshness_fusion freshness_expr IH).
 Qed.
 
-Lemma isnext_translate_equations {eqs: list Source.equation} {seed seed': ident} {pre_binders: list binder} {init_eqs step_eqs pre_eqs init_post step_post: list Target.equation}:
-  translate_equations eqs seed = (init_eqs, step_eqs, seed', pre_binders, pre_eqs, init_post, step_post)
-  -> forall x, In x (map fst pre_binders) -> exists n, x = iter n next_ident seed.
+Lemma isnext_translate_equations (eqs: list Source.equation) (seed: ident):
+  let '(init_eqs, step_eqs, seed', pre_binders, pre_eqs, init_post, step_post) := translate_equations eqs seed in
+  forall x, In x (map fst pre_binders) -> exists n, x = iter n next_ident seed.
 Proof.
-  intro translation.
+  destruct (translate_equations eqs seed) as [[[[[[init_eqs step_eqs] seed'] pre_binders] pre_eqs] init_post] step_post] eqn: translation.
   induction eqs as [| eq eqs IH] in seed, seed', pre_binders, init_eqs, step_eqs, pre_eqs, init_post, step_post, translation |- *.
   - injection translation as <- <- <- <- <- <- <-.
     intros.
     contradiction.
   - simpl in translation.
+    assert (nextseed := translate_equations_nextseed eqs seed).
     destruct (translate_equations eqs seed) as [[[[[[init_eqs0 step_eqs0] seed0] binders0] pre_eqs0] init_post0] step_post0] eqn: unfoldtrans.
     destruct eq as [ident [ty expr]].
-    destruct (translate_expr expr seed0) as [[[[[[ei2 es2] seed2] binders2] pre_eqs2] init_post2] step_post2] eqn: unfoldexpr.
+    assert (isnext_expr := isnext_translate_expr expr seed0).
+    destruct (translate_expr expr seed0) as [[[[[[ei2 es2] seed2] binders2] pre_eqs2] init_post2] step_post2].
     injection translation as <- <- <- <- <- <- <-.
     specialize (IH _ _ _ _ _ _ _ _ unfoldtrans).
     intros x isin.
     specialize (IH x).
-    assert (isnext_expr := isnext_translate_expr unfoldexpr).
-    assert (nextseed := translate_equations_nextseed unfoldtrans).
     destruct nextseed as [nseed nextseed].
     rewrite nextseed in isnext_expr.
     specialize (isnext_expr x).
@@ -213,49 +219,50 @@ Proof.
     assumption.
 Qed.
 
-Lemma nodup_translate_equations {eqs: list Source.equation} {seed seed': ident} {pre_binders: list binder} {init_eqs step_eqs pre_eqs init_post step_post: list Target.equation}:
-  translate_equations eqs seed = (init_eqs, step_eqs, seed', pre_binders, pre_eqs, init_post, step_post)
-  -> NoDup (map fst pre_binders).
+Lemma nodup_translate_equations (eqs: list Source.equation) (seed: ident):
+  let '(init_eqs, step_eqs, seed', pre_binders, pre_eqs, init_post, step_post) := translate_equations eqs seed in
+  NoDup (map fst pre_binders).
 Proof.
-  intro translation.
+  destruct (translate_equations eqs seed) as [[[[[[init_eqs step_eqs] seed'] pre_binders] pre_eqs] init_post] step_post] eqn: translation.
   induction eqs as [| eq eqs IH] in seed, seed', pre_binders, init_eqs, step_eqs, pre_eqs, init_post, step_post, translation |- *.
   - injection translation as <- <- <- <- <- <- <-.
     apply NoDup_nil.
   - simpl in translation.
+    assert (freshness_trans := freshness_translate_equations eqs seed).
     destruct (translate_equations eqs seed) as [[[[[[init_eqs0 step_eqs0] seed0] binders0] pre_eqs0] init_post0] step_post0] eqn: unfoldtrans.
     destruct eq as [ident [ty expr]].
-    destruct (translate_expr expr seed0) as [[[[[[ei2 es2] seed2] binders2] pre_eqs2] init_post2] step_post2] eqn: unfoldexpr.
+    assert (nodup_expr := nodup_translate_expr expr seed0).
+    assert (isnext := isnext_translate_expr expr seed0).
+    destruct (translate_expr expr seed0) as [[[[[[ei2 es2] seed2] binders2] pre_eqs2] init_post2] step_post2].
     injection translation as <- <- <- <- <- <- <-.
     specialize (IH _ _ _ _ _ _ _ _ unfoldtrans).
-    assert (nodup_expr := nodup_translate_expr unfoldexpr).
     rewrite map_app.
     apply NoDup_app.
     1, 2: assumption.
     intros x isin2.
     intro isin0.
-    assert (freshness_trans := freshness_translate_equations unfoldtrans).
-    assert (isnext := isnext_translate_expr unfoldexpr x isin2).
+    specialize (isnext  x isin2).
     destruct isnext as [n isnext].
     specialize (freshness_trans n).
     rewrite isnext in isin0.
     contradiction.
 Qed.
 
-Lemma translate_equations_assigned_init {eqs: list Source.equation} {seed seed': ident} {pre_binders: list binder} {init_eqs step_eqs pre_eqs init_post step_post: list Target.equation}:
-  translate_equations eqs seed = (init_eqs, step_eqs, seed', pre_binders, pre_eqs, init_post, step_post)
-  -> Permutation (map Target.equation_dest (pre_eqs ++ init_post)) pre_binders.
+Lemma translate_equations_assigned_init (eqs: list Source.equation) (seed: ident):
+  let '(init_eqs, step_eqs, seed', pre_binders, pre_eqs, init_post, step_post) := translate_equations eqs seed in
+  Permutation (map Target.equation_dest (pre_eqs ++ init_post)) pre_binders.
 Proof.
-  intro translation.
+  destruct (translate_equations eqs seed) as [[[[[[init_eqs step_eqs] seed'] pre_binders] pre_eqs] init_post] step_post] eqn: translation.
   induction eqs as [| eq eqs IH] in seed, seed', pre_binders, init_eqs, step_eqs, pre_eqs, init_post, step_post, translation |- *.
   - injection translation as <- <- <- <- <- <- <-.
     apply perm_nil.
   - simpl in translation.
     destruct (translate_equations eqs seed) as [[[[[[init_eqs0 step_eqs0] seed0] binders0] pre_eqs0] init_post0] step_post0] eqn: unfoldtrans.
     destruct eq as [ident [ty expr]].
-    destruct (translate_expr expr seed0) as [[[[[[ei2 es2] seed2] binders2] pre_eqs2] init_post2] step_post2] eqn: unfoldexpr.
+    assert (perm_expr := translate_expr_assigned_init expr seed0).
+    destruct (translate_expr expr seed0) as [[[[[[ei2 es2] seed2] binders2] pre_eqs2] init_post2] step_post2].
     injection translation as <- <- <- <- <- <- <-.
     specialize (IH _ _ _ _ _ _ _ _ unfoldtrans).
-    assert (perm_expr := translate_expr_assigned_init unfoldexpr).
     rewrite !map_app.
     rewrite map_app in IH.
     rewrite map_app in perm_expr.
@@ -269,21 +276,21 @@ Proof.
     all: assumption.
 Qed.
 
-Lemma translate_equations_assigned_step {eqs: list Source.equation} {seed seed': ident} {pre_binders: list binder} {init_eqs step_eqs pre_eqs init_post step_post: list Target.equation}:
-  translate_equations eqs seed = (init_eqs, step_eqs, seed', pre_binders, pre_eqs, init_post, step_post)
-  -> Permutation (map Target.equation_dest (pre_eqs ++ step_post)) pre_binders.
+Lemma translate_equations_assigned_step (eqs: list Source.equation) (seed: ident):
+  let '(init_eqs, step_eqs, seed', pre_binders, pre_eqs, init_post, step_post) := translate_equations eqs seed in
+  Permutation (map Target.equation_dest (pre_eqs ++ step_post)) pre_binders.
 Proof.
-  intro translation.
+  destruct (translate_equations eqs seed) as [[[[[[init_eqs step_eqs] seed'] pre_binders] pre_eqs] init_post] step_post] eqn: translation.
   induction eqs as [| eq eqs IH] in seed, seed', pre_binders, init_eqs, step_eqs, pre_eqs, init_post, step_post, translation |- *.
   - injection translation as <- <- <- <- <- <- <-.
     apply perm_nil.
   - simpl in translation.
     destruct (translate_equations eqs seed) as [[[[[[init_eqs0 step_eqs0] seed0] binders0] pre_eqs0] init_post0] step_post0] eqn: unfoldtrans.
     destruct eq as [ident [ty expr]].
-    destruct (translate_expr expr seed0) as [[[[[[ei2 es2] seed2] binders2] pre_eqs2] init_post2] step_post2] eqn: unfoldexpr.
+    assert (perm_expr := translate_expr_assigned_step expr seed0).
+    destruct (translate_expr expr seed0) as [[[[[[ei2 es2] seed2] binders2] pre_eqs2] init_post2] step_post2].
     injection translation as <- <- <- <- <- <- <-.
     specialize (IH _ _ _ _ _ _ _ _ unfoldtrans).
-    assert (perm_expr := translate_expr_assigned_step unfoldexpr).
     rewrite !map_app.
     rewrite map_app in IH.
     rewrite map_app in perm_expr.
@@ -297,18 +304,18 @@ Proof.
     all: assumption.
 Qed.
 
-Lemma translate_equations_conservation_init {eqs: list Source.equation} {seed seed': ident} {pre_binders: list binder} {init_eqs step_eqs pre_eqs init_post step_post: list Target.equation}:
-  translate_equations eqs seed = (init_eqs, step_eqs, seed', pre_binders, pre_eqs, init_post, step_post)
-  -> map Source.equation_dest eqs = map Target.equation_dest init_eqs.
+Lemma translate_equations_conservation_init (eqs: list Source.equation) (seed: ident):
+  let '(init_eqs, step_eqs, seed', pre_binders, pre_eqs, init_post, step_post) := translate_equations eqs seed in
+  map Source.equation_dest eqs = map Target.equation_dest init_eqs.
 Proof.
-  intro translation.
+  destruct (translate_equations eqs seed) as [[[[[[init_eqs step_eqs] seed'] pre_binders] pre_eqs] init_post] step_post] eqn: translation.
   induction eqs as [| eq eqs IH] in seed, seed', pre_binders, init_eqs, step_eqs, pre_eqs, init_post, step_post, translation |- *.
   - injection translation as <- <- <- <- <- <- <-.
     reflexivity.
   - simpl in translation.
     destruct (translate_equations eqs seed) as [[[[[[init_eqs0 step_eqs0] seed0] binders0] pre_eqs0] init_post0] step_post0] eqn: unfoldtrans.
     destruct eq as [ident [ty expr]].
-    destruct (translate_expr expr seed0) as [[[[[[ei2 es2] seed2] binders2] pre_eqs2] init_post2] step_post2] eqn: unfoldexpr.
+    destruct (translate_expr expr seed0) as [[[[[[ei2 es2] seed2] binders2] pre_eqs2] init_post2] step_post2].
     injection translation as <- <- <- <- <- <- <-.
     specialize (IH _ _ _ _ _ _ _ _ unfoldtrans).
     rewrite !map_cons.
@@ -317,18 +324,18 @@ Proof.
     reflexivity.
 Qed.
 
-Lemma translate_equations_conservation_step {eqs: list Source.equation} {seed seed': ident} {pre_binders: list binder} {init_eqs step_eqs pre_eqs init_post step_post: list Target.equation}:
-  translate_equations eqs seed = (init_eqs, step_eqs, seed', pre_binders, pre_eqs, init_post, step_post)
-  -> map Source.equation_dest eqs = map Target.equation_dest step_eqs.
+Lemma translate_equations_conservation_step (eqs: list Source.equation) (seed: ident):
+  let '(init_eqs, step_eqs, seed', pre_binders, pre_eqs, init_post, step_post) := translate_equations eqs seed in
+  map Source.equation_dest eqs = map Target.equation_dest step_eqs.
 Proof.
-  intro translation.
+  destruct (translate_equations eqs seed) as [[[[[[init_eqs step_eqs] seed'] pre_binders] pre_eqs] init_post] step_post] eqn: translation.
   induction eqs as [| eq eqs IH] in seed, seed', pre_binders, init_eqs, step_eqs, pre_eqs, init_post, step_post, translation |- *.
   - injection translation as <- <- <- <- <- <- <-.
     reflexivity.
   - simpl in translation.
     destruct (translate_equations eqs seed) as [[[[[[init_eqs0 step_eqs0] seed0] binders0] pre_eqs0] init_post0] step_post0] eqn: unfoldtrans.
     destruct eq as [ident [ty expr]].
-    destruct (translate_expr expr seed0) as [[[[[[ei2 es2] seed2] binders2] pre_eqs2] init_post2] step_post2] eqn: unfoldexpr.
+    destruct (translate_expr expr seed0) as [[[[[[ei2 es2] seed2] binders2] pre_eqs2] init_post2] step_post2].
     injection translation as <- <- <- <- <- <- <-.
     specialize (IH _ _ _ _ _ _ _ _ unfoldtrans).
     rewrite !map_cons.
@@ -336,6 +343,141 @@ Proof.
     rewrite IH.
     reflexivity.
 Qed.
+
+Lemma translate_init_assigned {n_body n_out n_locals} (n_seed: ident)
+  (n_vars_all_assigned : Permutation (map Source.equation_dest n_body) (n_out ++ n_locals)) :
+  let '(init_eqs, step_eqs, new_seed, pre_binders, pre_eqs, init_post_eqs, step_post_eqs) := translate_equations n_body n_seed in
+  Permutation (map Target.equation_dest pre_eqs ++ map Target.equation_dest (init_eqs ++ init_post_eqs)) (n_out ++ pre_binders ++ n_locals).
+Proof.
+  assert (conservation_init := translate_equations_conservation_init n_body n_seed).
+  assert (assigned_init := translate_equations_assigned_init n_body n_seed).
+  destruct (translate_equations n_body n_seed) as [[[[[[init_eqs step_eqs] seed'] pre_binders] pre_eqs] init_post] step_post].
+  rewrite map_app.
+  rewrite <- conservation_init.
+  rewrite (Permutation_app_comm (map Source.equation_dest n_body)).
+  rewrite !app_assoc.
+  rewrite (Permutation_app_comm n_out).
+  rewrite <- !app_assoc.
+  rewrite <- n_vars_all_assigned.
+  rewrite !app_assoc.
+  apply Permutation_app.
+  2: apply Permutation_refl.
+  rewrite <- map_app.
+  assumption.
+Qed.
+
+Lemma translate_step_assigned {n_body n_out n_locals} (n_seed: ident)
+  (n_vars_all_assigned : Permutation (map Source.equation_dest n_body) (n_out ++ n_locals)) :
+  let '(init_eqs, step_eqs, new_seed, pre_binders, pre_eqs, init_post_eqs, step_post_eqs) := translate_equations n_body n_seed in
+  Permutation (map Target.equation_dest pre_eqs ++ map Target.equation_dest (step_eqs ++ step_post_eqs)) (n_out ++ pre_binders ++ n_locals).
+Proof.
+  assert (conservation_step := translate_equations_conservation_step n_body n_seed).
+  assert (assigned_step := translate_equations_assigned_step n_body n_seed).
+  destruct (translate_equations n_body n_seed) as [[[[[[init_eqs step_eqs] seed'] pre_binders] pre_eqs] init_post] step_post].
+  rewrite map_app.
+  rewrite <- conservation_step.
+  rewrite (Permutation_app_comm (map Source.equation_dest n_body)).
+  rewrite !app_assoc.
+  rewrite (Permutation_app_comm n_out).
+  rewrite <- !app_assoc.
+  rewrite <- n_vars_all_assigned.
+  rewrite !app_assoc.
+  apply Permutation_app.
+  2: apply Permutation_refl.
+  rewrite <- map_app.
+  assumption.
+Qed.
+
+Lemma translate_vars_unique {n_in n_out n_locals n_seed} (n_body: list Source.equation)
+  (n_vars_unique : NoDup (map fst (n_in ++ n_out ++ n_locals)))
+  (n_seed_always_fresh : freshness n_seed (n_in ++ n_out ++ n_locals)) :
+  let '(init_eqs, step_eqs, new_seed, pre_binders, pre_eqs, init_post_eqs, step_post_eqs) := translate_equations n_body n_seed in
+  NoDup (map fst (n_in ++ n_out ++ pre_binders ++ n_locals)).
+Proof.
+  assert (nodup_translate := nodup_translate_equations n_body n_seed).
+  assert (isnext := isnext_translate_equations n_body n_seed).
+  destruct (translate_equations n_body n_seed) as [[[[[[init_eqs step_eqs] seed'] pre_binders] pre_eqs] init_post] step_post].
+  rewrite !map_app.
+  rewrite !map_app in n_vars_unique.
+  unfold freshness in n_seed_always_fresh.
+  rewrite !map_app in n_seed_always_fresh.
+  rewrite app_assoc.
+  rewrite Permutation_app_comm.
+  rewrite (Permutation_app_comm (map fst pre_binders)).
+  rewrite <- app_assoc.
+  rewrite Permutation_app_comm.
+  rewrite <- !app_assoc.
+  apply NoDup_app.
+  1, 2: assumption.
+  intros x isin.
+  specialize (isnext x isin).
+  destruct isnext as [n isnext].
+  rewrite isnext.
+  apply (n_seed_always_fresh n).
+Qed.
+
+Lemma translate_seed_always_fresh {n_in n_out n_locals n_seed} (n_body: list Source.equation)
+  (n_seed_always_fresh : freshness n_seed (n_in ++ n_out ++ n_locals)) :
+  let '(init_eqs, step_eqs, new_seed, pre_binders, pre_eqs, init_post_eqs, step_post_eqs) := translate_equations n_body n_seed in
+  freshness new_seed (n_in ++ n_out ++ pre_binders ++ n_locals).
+Proof.
+  assert (fresh_translate := freshness_translate_equations n_body n_seed).
+  assert (nextseed := translate_equations_nextseed n_body n_seed).
+  destruct (translate_equations n_body n_seed) as [[[[[[init_eqs step_eqs] seed'] pre_binders] pre_eqs] init_post] step_post].
+  intros n isin.
+  rewrite !map_app in isin.
+  unfold freshness in n_seed_always_fresh.
+  rewrite !map_app in n_seed_always_fresh.
+  rewrite app_assoc in isin.
+  rewrite Permutation_app_comm in isin.
+  rewrite (Permutation_app_comm (map fst pre_binders)) in isin.
+  rewrite <- app_assoc in isin.
+  rewrite Permutation_app_comm in isin.
+  rewrite <- !app_assoc in isin.
+  apply in_app_or in isin.
+  destruct nextseed as [nseed nextseed].
+  specialize (fresh_translate n).
+  destruct isin as [isin | isin].
+  1: contradiction.
+  rewrite nextseed in isin.
+  rewrite <- Nat.iter_add in isin.
+  specialize (n_seed_always_fresh (n + nseed)).
+  contradiction.
+Qed.
+
+Lemma translation_conservation n_seed n_body eq:
+  In eq n_body ->
+  let '(init_eqs, step_eqs, new_seed, pre_binders, pre_eqs, init_post_eqs, step_post_eqs) := translate_equations n_body n_seed in
+  let '(ident, existT _ ty e) := eq in
+  exists seed1,
+  let '(ei, es, seed2, pre_binders1, pre_eqs1, init_post1, step_post1) := translate_expr e seed1 in
+    In (ident, existT _ ty ei) init_eqs /\
+    In (ident, existT _ ty es) step_eqs.
+Proof.
+  induction n_body as [|eq' n_body IH].
+  1: contradiction.
+  simpl.
+  destruct (translate_equations n_body n_seed) as [[[[[[init_eqs step_eqs] seed'] pre_binders] pre_eqs] init_post] step_post].
+  intros [|isin]; subst.
+  all: destruct eq as [ident [ty e]].
+  - destruct (translate_expr e seed') as [[[[[[ei1 es1] seed1] binders1] pre_eqs1] init_post1] step_post1] eqn: translation.
+    exists seed'.
+    destruct (translate_expr e seed') as [[[[[[]]]]]].
+    injection translation as <- <- <- <- <- <- <-.
+    split.
+    all: constructor 1.
+    all: reflexivity.
+  - destruct eq' as [ident' [ty' e']].
+    specialize (IH isin).
+    destruct IH as [seed1 IH].
+    destruct (translate_expr e' seed') as [[[[[[]]]]]].
+    exists seed1.
+    destruct (translate_expr e seed1) as [[[[[[]]]]]].
+    destruct IH.
+    split.
+    all: constructor 2; assumption.
+Qed.
+
 
 Definition translate_node (node: Source.node) : Result.t type Target.node.
 Proof.
@@ -360,6 +502,10 @@ Proof.
     n_seed
     n_seed_always_fresh
   ].
+  assert (init_assigned := translate_init_assigned n_seed n_vars_all_assigned).
+  assert (step_assigned := translate_step_assigned n_seed n_vars_all_assigned).
+  assert (vars_unique := translate_vars_unique n_body n_vars_unique n_seed_always_fresh).
+  assert (fresh_seed := translate_seed_always_fresh n_body n_seed_always_fresh).
 
   destruct (translate_equations n_body n_seed) as [
     [[[[[init_eqs
@@ -369,7 +515,7 @@ Proof.
     pre_eqs]
     init_post_eqs]
     step_post_eqs
-  ] eqn: translation.
+  ].
 
   refine {|
     Target.n_loc := n_loc;
@@ -384,70 +530,46 @@ Proof.
 
     Target.n_seed := new_seed;
   |}.
+  all: assumption.
+Defined.
 
-  all: subst n_vars n_assigned_vars.
 
-  - rewrite map_app.
-    rewrite <- (translate_equations_conservation_init translation).
-    rewrite (Permutation_app_comm (map Source.equation_dest n_body)).
-    rewrite !app_assoc.
-    rewrite (Permutation_app_comm n_out).
-    rewrite <- !app_assoc.
-    rewrite <- n_vars_all_assigned.
-    rewrite !app_assoc.
-    apply Permutation_app.
-    2: apply Permutation_refl.
-    rewrite <- map_app.
-    apply (translate_equations_assigned_init translation).
-  - rewrite map_app.
-    rewrite <- (translate_equations_conservation_step translation).
-    rewrite (Permutation_app_comm (map Source.equation_dest n_body)).
-    rewrite !app_assoc.
-    rewrite (Permutation_app_comm n_out).
-    rewrite <- !app_assoc.
-    rewrite <- n_vars_all_assigned.
-    rewrite !app_assoc.
-    apply Permutation_app.
-    2: apply Permutation_refl.
-    rewrite <- map_app.
-    apply (translate_equations_assigned_step translation).
-  - rewrite !map_app.
-    rewrite !map_app in n_vars_unique.
-    unfold freshness in n_seed_always_fresh.
-    rewrite !map_app in n_seed_always_fresh.
-    rewrite app_assoc.
-    rewrite Permutation_app_comm.
-    rewrite (Permutation_app_comm (map fst pre_binders)).
-    rewrite <- app_assoc.
-    rewrite Permutation_app_comm.
-    rewrite <- !app_assoc.
-    apply NoDup_app.
-    1: apply (nodup_translate_equations translation).
-    1: assumption.
-    intros x isin.
-    assert (isnext := isnext_translate_equations translation x isin).
-    destruct isnext as [n isnext].
-    rewrite isnext.
-    apply (n_seed_always_fresh n).
-  - intros n isin.
-    rewrite !map_app in isin.
-    unfold freshness in n_seed_always_fresh.
-    rewrite !map_app in n_seed_always_fresh.
-    rewrite app_assoc in isin.
-    rewrite Permutation_app_comm in isin.
-    rewrite (Permutation_app_comm (map fst pre_binders)) in isin.
-    rewrite <- app_assoc in isin.
-    rewrite Permutation_app_comm in isin.
-    rewrite <- !app_assoc in isin.
-    apply in_app_or in isin.
-    assert (fresh_translate := freshness_translate_equations translation).
-    assert (nextseed := translate_equations_nextseed translation).
-    destruct nextseed as [nseed nextseed].
-    specialize (fresh_translate n).
-    destruct isin as [isin | isin].
-    1: contradiction.
-    rewrite nextseed in isin.
-    rewrite <- Nat.iter_add in isin.
-    specialize (n_seed_always_fresh (n + nseed)).
-    contradiction.
-Defined. 
+(* Semantics preservation *)
+Theorem semantics_preservation_inv (n: Target.node) (n0: Source.node) (h: history):
+  translate_node n0 = Result.Ok n -> Target.sem_node n h -> Source.sem_node n0 h.
+Proof.
+  intro translated.
+  unfold translate_node in translated.
+  apply Result.ok_eq in translated.
+  destruct n0 as [n0_loc n0_name n0_in n0_out n0_locals n0_body n0_vars n0_assigned_vars n0_all_vars_exist n0_vars_all_assigned n0_vars_unique n0_seed n0_seed_always_fresh].
+  remember (translate_init_assigned n0_seed n0_vars_all_assigned) as init_assigned eqn: tmp; clear tmp.
+  remember (translate_step_assigned n0_seed n0_vars_all_assigned) as step_assigned eqn: tmp; clear tmp.
+  remember (translate_vars_unique n0_body n0_vars_unique n0_seed_always_fresh) as vars_unique eqn: tmp; clear tmp.
+  remember (translate_seed_always_fresh n0_body n0_seed_always_fresh) as seed_fresh eqn: tmp; clear tmp.
+  destruct (translate_equations n0_body n0_seed) as [[[[[[trans_init trans_step] trans_seed] trans_pre_binders] trans_pre_eqs] trans_init_eqs] trans_step_eqs] eqn: translation.
+  subst.
+  unfold Source.sem_node, Target.sem_node, Target.n_vars, Target.n_init, Target.n_in, Target.n_out, Target.n_locals, Target.n_step, Target.n_pre, Source.n_body.
+
+  intro sem_target.
+  intros idn ty expr s inbody ismapped time.
+
+  specialize (sem_target idn ty).
+  assert (id_is_var : In (idn, ty) (n0_in ++ n0_out ++ trans_pre_binders ++ n0_locals)).
+  {
+   assert (id_is_var2 : In (idn, ty) (n0_out ++ n0_locals)).
+   2: apply in_or_app; right; apply in_or_app.
+   2: apply in_app_or in id_is_var2; destruct id_is_var2.
+   2: left; assumption.
+   2: right; apply in_or_app; right; assumption.
+   rewrite <- n0_vars_all_assigned.
+   unfold n0_assigned_vars.
+   apply (in_map Source.equation_dest) in inbody.
+   unfold Source.equation_dest at 1 in inbody.
+   unfold fst, snd, projT1 in inbody.
+   assumption.
+  }
+
+  specialize (sem_target id_is_var).
+  destruct sem_target as [s' [ismapped' sem_target]].
+  
+Admitted.
